typed-assembly/ControlFlow.v
@@ -1,0 +1,98 @@
+(** Experiments to find a nice representation of an annoted control-flow graph *)
+Require Import Wellfounded.
+
+Set Implicit Arguments.
+
+Module WellFounded.
+  Record t (A : Type) : Type := new {
+    lt : A -> A -> Prop;
+    Hwf : well_founded lt}.
+End WellFounded.
+
+Module Context.
+  Module T.
+    Inductive t (S : Set) : Type :=
+    | nil
+    | cons (A : Type) (WF : WellFounded.t A) (C : t S).
+    
+    Fixpoint append S (C1 C2 : t S) : t S :=
+      match C1 with
+      | nil _ => C2
+      | cons WF C1 => cons WF (append C1 C2)
+      end.
+  End T.
+  
+  Module I.
+    Inductive t (S : Set) : T.t S -> Type :=
+    | nil : t (T.nil S)
+    | cons : forall A WF (C : T.t S) (a : A) (c : t C), t (T.cons (A := A) WF C).
+  End I.
+  
+  Inductive lt S : {C : T.t S & I.t C} -> {C : T.t S & I.t C} -> Prop :=
+  | lt_nil : forall A WF a C c,
+    lt (existT _ _ (I.cons (A := A) WF (C := C) a c))
+       (existT _ _ (I.nil S))
+  | lt_head_lt : forall A WF a1 a2 C1 C2 c1 c2,
+    WellFounded.lt WF a1 a2 ->
+    lt (existT _ _ (I.cons (A := A) WF (C := C1) a1 c1))
+       (existT _ _ (I.cons (A := A) WF (C := C2) a2 c2))
+  | lt_head_eq : forall A WF a C1 C2 c1 c2,
+    lt (existT _ _ c1)
+       (existT _ _ c2) ->
+    lt (existT _ _ (I.cons (A := A) WF (C := C1) a c1))
+       (existT _ _ (I.cons (A := A) WF (C := C2) a c2)).
+  
+  Lemma lt_wf (S : Set) : well_founded (lt (S := S)).
+    intro x.
+    constructor; intros y H.
+  Admitted.
+End Context.
+
+Module CFG.
+  Inductive t (S : Set) : Context.t S -> (S -> Type) -> (S -> Type) -> Type :=
+  | nop : forall C L,
+    t C L L
+  | op : forall C Lin L Lout,
+    (forall s, {s' : S & Lin s -> L s'}) ->
+    t C L Lout ->
+    t C Lin Lout
+  | jcc : forall C Lin Lin_true Lin_false Lmerge Lout,
+    (forall s, (Lin s -> Lin_true s) + (Lin s -> Lin_false s)) ->
+    t C Lin_true Lmerge -> t C Lin_false Lmerge -> t C Lmerge Lout ->
+    t C Lin Lout
+  | label : forall C Lin L Lout (WF : WellFounded.t (sigT Lin)),
+    t (Context.cons WF C) Lin L -> t C L Lout ->
+    t C Lin Lout
+  | goto : forall C1 C2 Lin L Lout (WF : WellFounded.t (sigT Lin)),
+    
+    t (Context.append C1 (Context.cons WF C2)) Lin Lout.
+  
+  (*Inductive t (S : Set) : (S -> Type) -> (S -> Type) -> Type :=
+  | op : forall (f : S -> S) (Lin L Lout : S -> Type)
+    (fl : forall s, Lin s -> L (f s)),
+    t S L Lout ->
+    t S Lin Lout
+  | jcc : forall (c : S -> bool) (Lin Lin_true Lin_false Lmerge Lout : S -> Type)
+    (fl : forall s, if c s then Lin s -> Lin_true s else Lin s -> Lin_false s),
+    t S Lin_true Lmerge -> t S Lin_false Lmerge -> t S Lmerge Lout ->
+    t S Lin Lout.*)
+  
+  Fixpoint eval S Lin Lout (p : t S Lin Lout)
+    (s : S) (l : Lin s) {struct p} : {s' : S & Lout s'}.
+    destruct p as [Lin L Lout f p
+      | Lin Lin_true Lin_false Lmerge Lout f p_true p_false p].
+    - exact (
+        let (_, fl) := f s in
+        eval _ _ _ p _ (fl l)).
+    
+    - exact (
+        match f s with
+        | inl fl_true =>
+          let (s, l) := eval _ _ _ p_true _ (fl_true l) in
+          eval _ _ _ p _ l
+        | inr fl_false =>
+          let (s, l) := eval _ _ _ p_false _ (fl_false l) in
+          eval _ _ _ p _ l
+        end).
+  Defined.
+End CFG.
